imp/ImpProofs.v
@@ -150,7 +150,7 @@ Section PROOFS.
       if (call_mem f)
       then triggerUB
       else
-        eval_args <- (denote_exprs args []);;
+        eval_args <- (denote_exprs args);;
         v <- trigger (Call f (eval_args↑));; v <- unwrapN (v↓);;
         trigger (SetVar x v);;; Ret Vundef).
   Proof. reflexivity. Qed.
@@ -164,7 +164,7 @@ Section PROOFS.
       if (call_mem f)
       then triggerUB
       else
-        eval_args <- (denote_exprs args []);;
+        eval_args <- (denote_exprs args);;
         v <- trigger (Call f (eval_args↑));; v <- unwrapN (v↓);;
         trigger (SetVar x v);;; Ret Vundef).
   Proof. reflexivity. Qed.
@@ -174,7 +174,7 @@ Section PROOFS.
     :
       interp_imp ge le0 (denote_stmt (CallSys x f args)) =
       interp_imp ge le0 (
-      eval_args <- (denote_exprs args []);;
+      eval_args <- (denote_exprs args);;
       v <- trigger (Syscall f eval_args top1);;
       trigger (SetVar x v);;; Ret Vundef).
   Proof. reflexivity. Qed.
@@ -545,53 +545,102 @@ Section PROOFS.
     apply interp_imp_Call_ret.
   Qed.
 
-  Fixpoint interp_imp_denote_exprs ge le es acc :=
-    match es with
-    | [] => Ret (le, acc)
-    | e :: s =>
-      '(le1, v) <- interp_imp ge le (denote_expr e);;
-      interp_imp_denote_exprs ge le1 s (acc ++ [v])
-    end.
+  (* Fixpoint interp_imp_denote_exprs ge le es acc := *)
+  (*   match es with *)
+  (*   | [] => Ret (le, acc) *)
+  (*   | e :: s => *)
+  (*     '(le1, v) <- interp_imp ge le (denote_expr e);; *)
+  (*     interp_imp_denote_exprs ge le1 s (acc ++ [v]) *)
+  (*   end. *)
 
-  Lemma interp_imp_exprs
-        ge le0 x f args acc
+  (* Lemma interp_imp_exprs *)
+  (*       ge le0 x f args acc *)
+  (*   : *)
+  (*     interp_imp ge le0 ( *)
+  (*                  eval_args <- (denote_exprs args acc);; *)
+  (*                  v <- trigger (Call f (eval_args↑));; v <- unwrapN (v↓);; *)
+  (*                  trigger (SetVar x v);; Ret Vundef) *)
+  (*     = *)
+  (*     '(le1, vs) <- interp_imp_denote_exprs ge le0 args acc;; *)
+  (*     v <- trigger (Call f (vs↑));; *)
+  (*     tau;; tau;; v <- unwrapN (v↓);; *)
+  (*     tau;; tau;; Ret (alist_add x v le1, Vundef). *)
+  (* Proof. *)
+  (*   move args before Σ. revert_until args. induction args; i. *)
+  (*   - grind. apply interp_imp_Call_ret. *)
+  (*   - grind. rewrite interp_imp_bind. grind. *)
+  (*     destruct x0. auto. *)
+  (* Qed. *)
+
+  Lemma interp_imp_Call_nil
+        ge le0 x f
     :
       interp_imp ge le0 (
-                   eval_args <- (denote_exprs args acc);;
+                   eval_args <- (denote_exprs []);;
+                   v <- trigger (Call f ((eval_args)↑));; v <- unwrapN (v↓);;
+                   trigger (SetVar x v);; Ret Vundef)
+      =
+      v <- trigger (Call f (([]: list val)↑));;
+      tau;; tau;; v <- unwrapN (v↓);;
+      tau;; tau;; Ret (alist_add x v le0, Vundef).
+  Proof.
+    rewrite <- (interp_imp_Call_ret ge le0 f _ x). ss. grind.
+  Qed.
+
+  Lemma interp_imp_Call_args
+        ge le0 x f argsh argst
+    :
+      interp_imp ge le0 (
+                   eval_args <- (denote_exprs (argsh :: argst));;
                    v <- trigger (Call f (eval_args↑));; v <- unwrapN (v↓);;
                    trigger (SetVar x v);;; Ret Vundef)
       =
-      '(le1, vs) <- interp_imp_denote_exprs ge le0 args acc;;
-      v <- trigger (Call f (vs↑));;
-      tau;; tau;; v <- unwrapN (v↓);;
-      tau;; tau;; Ret (alist_add x v le1, Vundef).
+      '(le1, vh) <- interp_imp ge le0 (denote_expr argsh);;
+      interp_imp ge le1 (
+                   eval_args <- (denote_exprs argst);;
+                   v <- trigger (Call f ((vh :: eval_args)↑));; v <- unwrapN (v↓);;
+                   trigger (SetVar x v);; Ret Vundef).
   Proof.
-    move args before Σ. revert_until args. induction args; i.
-    - grind. apply interp_imp_Call_ret.
-    - grind. rewrite interp_imp_bind. grind.
-      destruct x0. auto.
+    ss. grind. rewrite interp_imp_bind. grind.
+    unfold interp_imp, interp_GlobEnv, interp_ImpState. grind.
   Qed.
 
-  Lemma interp_imp_CallFun
-        ge le0 x f args
+  Lemma interp_imp_CallFun_nil
+        ge le0 x f
     :
-      interp_imp ge le0 (denote_stmt (CallFun x f args)) =
+      interp_imp ge le0 (denote_stmt (CallFun x f [])) =
       if (call_mem f)
       then triggerUB
       else
-        '(le1, vs) <- interp_imp_denote_exprs ge le0 args [];;
-        v <- trigger (Call f (vs↑));;
+        v <- trigger (Call f (([]: list val)↑));;
         tau;; tau;; v <- unwrapN (v↓);;
-        tau;; tau;; Ret (alist_add x v le1, Vundef).
+        tau;; tau;; Ret (alist_add x v le0, Vundef).
   Proof.
-    rewrite denote_stmt_CallFun. des_ifs; try (apply interp_imp_exprs).
+    rewrite denote_stmt_CallFun. des_ifs; try (apply interp_imp_Call_nil).
     apply interp_imp_triggerUB.
   Qed.
 
-  Lemma interp_imp_CallPtr
-        ge le0 x e args
+  Lemma interp_imp_CallFun_args
+        ge le0 x f argsh argst
     :
-      interp_imp ge le0 (denote_stmt (CallPtr x e args)) =
+      interp_imp ge le0 (denote_stmt (CallFun x f (argsh :: argst))) =
+      if (call_mem f)
+      then triggerUB
+      else
+        '(le1, vh) <- interp_imp ge le0 (denote_expr argsh);;
+        interp_imp ge le1 (
+                     eval_args <- (denote_exprs argst);;
+                     v <- trigger (Call f ((vh :: eval_args)↑));; v <- unwrapN (v↓);;
+                     trigger (SetVar x v);; Ret Vundef).
+  Proof.
+    rewrite denote_stmt_CallFun. des_ifs; try (apply interp_imp_Call_args).
+    apply interp_imp_triggerUB.
+  Qed.
+
+  Lemma interp_imp_CallPtr_nil
+        ge le0 x e
+    :
+      interp_imp ge le0 (denote_stmt (CallPtr x e [])) =
       '(le1, p) <- interp_imp ge le0 (denote_expr e);;
       match p with
       | Vptr n 0 =>
@@ -601,10 +650,9 @@ Section PROOFS.
           then tau;; triggerUB
           else
             tau;;
-            '(le2, vs) <- interp_imp_denote_exprs ge le1 args [];;
-            v <- trigger (Call f (vs↑));;
+            v <- trigger (Call f (([]: list val)↑));;
             tau;; tau;; v <- unwrapN (v↓);;
-            tau;; tau;; Ret (alist_add x v le2, Vundef)
+            tau;; tau;; Ret (alist_add x v le1, Vundef)
         | None => triggerUB
         end
       | _ => triggerUB
@@ -615,39 +663,115 @@ Section PROOFS.
     des_ifs; rewrite interp_trigger; grind.
     all:( unfold triggerUB, unwrapU, pure_state; grind).
     - rewrite interp_trigger; grind.
-    - rewrite <- (interp_imp_exprs ge) with (acc := []).
+    - rewrite <- (interp_imp_Call_nil ge).
       unfold interp_imp, interp_GlobEnv, interp_ImpState. grind.
     - unfold triggerUB. grind.
   Qed.
 
-  Lemma interp_imp_exprs_sys
-        ge le0 x f args acc
+  Lemma interp_imp_CallPtr_args
+        ge le0 x e argsh argst
+    :
+      interp_imp ge le0 (denote_stmt (CallPtr x e (argsh :: argst))) =
+      '(le1, p) <- interp_imp ge le0 (denote_expr e);;
+      match p with
+      | Vptr n 0 =>
+        match (SkEnv.blk2id ge n) with
+        | Some f =>
+          if (call_mem f)
+          then tau;; triggerUB
+          else
+            tau;;
+            '(le2, vh) <- interp_imp ge le1 (denote_expr argsh);;
+            interp_imp ge le2 (
+                         eval_args <- (denote_exprs argst);;
+                         v <- trigger (Call f ((vh :: eval_args)↑));; v <- unwrapN (v↓);;
+                         trigger (SetVar x v);; Ret Vundef)
+      | None => triggerUB
+        end
+      | _ => triggerUB
+      end.
+  Proof.
+    rewrite denote_stmt_CallPtr. rewrite interp_imp_bind. grind.
+    unfold interp_imp, interp_GlobEnv, interp_ImpState. grind.
+    des_ifs; rewrite interp_trigger; grind.
+    all:( unfold triggerUB, unwrapU, pure_state; grind).
+    - rewrite interp_trigger; grind.
+    - unfold triggerUB. grind.
+  Qed.
+
+  (* Lemma interp_imp_exprs_sys *)
+  (*       ge le0 x f args acc *)
+  (*   : *)
+  (*     interp_imp ge le0 ( *)
+  (*                  eval_args <- (denote_exprs args acc);; *)
+  (*                  v <- trigger (Syscall f eval_args top1);; *)
+  (*                  trigger (SetVar x v);; Ret Vundef) *)
+  (*     = *)
+  (*     '(le1, vs) <- interp_imp_denote_exprs ge le0 args acc;; *)
+  (*     v <- trigger (Syscall f vs top1);; *)
+  (*     tau;; tau;; tau;; tau;; *)
+  (*     Ret (alist_add x v le1, Vundef). *)
+  (* Proof. *)
+  (*   move args before Σ. revert_until args. induction args; i. *)
+  (*   - grind. apply interp_imp_Syscall_ret. *)
+  (*   - grind. rewrite interp_imp_bind. grind. destruct x0. auto. *)
+  (* Qed. *)
+
+  Lemma interp_imp_Syscall_nil
+        ge le0 x f
     :
       interp_imp ge le0 (
-                   eval_args <- (denote_exprs args acc);;
+                   eval_args <- (denote_exprs []);;
                    v <- trigger (Syscall f eval_args top1);;
                    trigger (SetVar x v);;; Ret Vundef)
       =
-      '(le1, vs) <- interp_imp_denote_exprs ge le0 args acc;;
-      v <- trigger (Syscall f vs top1);;
+      v <- trigger (Syscall f ([]: list val) top1);;
       tau;; tau;; tau;; tau;;
-      Ret (alist_add x v le1, Vundef).
+      Ret (alist_add x v le0, Vundef).
   Proof.
-    move args before Σ. revert_until args. induction args; i.
-    - grind. apply interp_imp_Syscall_ret.
-    - grind. rewrite interp_imp_bind. grind. destruct x0. auto.
+    rewrite <- (interp_imp_Syscall_ret ge le0 f _ x). ss. grind.
   Qed.
 
-  Lemma interp_imp_CallSys
-        ge le0 x f args
+  Lemma interp_imp_Syscall_args
+        ge le0 x f argsh argst
     :
-      interp_imp ge le0 (denote_stmt (CallSys x f args)) =
-      '(le1, vs) <- interp_imp_denote_exprs ge le0 args [];;
-      v <- trigger (Syscall f vs top1);;
-      tau;; tau;; tau;; tau;;
-      Ret (alist_add x v le1, Vundef).
+      interp_imp ge le0 (
+                   eval_args <- (denote_exprs (argsh :: argst));;
+                   v <- trigger (Syscall f eval_args top1);;
+                   trigger (SetVar x v);; Ret Vundef)
+      =
+      '(le1, vh) <- interp_imp ge le0 (denote_expr argsh);;
+      interp_imp ge le1 (
+                   eval_args <- (denote_exprs argst);;
+                   v <- trigger (Syscall f (vh :: eval_args) top1);;
+                   trigger (SetVar x v);; Ret Vundef).
   Proof.
-    rewrite denote_stmt_CallSys. apply interp_imp_exprs_sys.
+    ss. grind. rewrite interp_imp_bind. grind.
+    unfold interp_imp, interp_GlobEnv, interp_ImpState. grind.
+  Qed.
+
+  Lemma interp_imp_CallSys_nil
+        ge le0 x f
+    :
+      interp_imp ge le0 (denote_stmt (CallSys x f [])) =
+        v <- trigger (Syscall f ([]: list val) top1);;
+        tau;; tau;; tau;; tau;;
+        Ret (alist_add x v le0, Vundef).
+  Proof.
+    rewrite denote_stmt_CallSys. des_ifs; try (apply interp_imp_Syscall_nil).
+  Qed.
+
+  Lemma interp_imp_CallSys_args
+        ge le0 x f argsh argst
+    :
+      interp_imp ge le0 (denote_stmt (CallSys x f (argsh :: argst))) =
+        '(le1, vh) <- interp_imp ge le0 (denote_expr argsh);;
+        interp_imp ge le1 (
+                     eval_args <- (denote_exprs argst);;
+                     v <- trigger (Syscall f (vh :: eval_args) top1);;
+                     trigger (SetVar x v);; Ret Vundef).
+  Proof.
+    rewrite denote_stmt_CallSys. des_ifs; try (apply interp_imp_Syscall_args).
   Qed.
 
   (* eval_imp  *)
@@ -693,9 +817,21 @@ Ltac imp_red :=
     | Assign _ _ => rewrite interp_imp_Assign
     | Seq _ _ => rewrite interp_imp_Seq; imp_red
     | If _ _ _ => rewrite interp_imp_If
-    | CallFun _ _ _ => rewrite interp_imp_CallFun
-    | CallPtr _ _ _ => rewrite interp_imp_CallPtr
-    | CallSys _ _ _ => rewrite interp_imp_CallSys
+    | CallFun _ _ ?args =>
+      match args with
+      | [] => rewrite interp_imp_CallFun_nil
+      | _ => rewrite interp_imp_CallFun_args; try (repeat (rewrite interp_imp_Call_args))
+      end
+    | CallPtr _ _ ?args =>
+      match args with
+      | [] => rewrite interp_imp_CallPtr_nil
+      | _ => rewrite interp_imp_CallPtr_args; try (repeat (rewrite interp_imp_Call_args))
+      end
+    | CallSys _ _ ?args =>
+      match args with
+      | [] => rewrite interp_imp_Syscall_nil
+      | _ => rewrite interp_imp_Syscall_args; try (repeat (rewrite interp_imp_Syscall_args))
+      end
     | AddrOf _ _ => rewrite interp_imp_AddrOf
     | Malloc _ _ => rewrite interp_imp_Malloc
     | Free _ => rewrite interp_imp_Free
